# Example
- #### Let $B=((1,1),(1,-1))$ and $C=((1,2),(1,3))$ find the change of basis matrix $,P_{B\to C}$
$$
\begin{align}
[\vec{v}_{1}]_{c}=? \\ 
\begin{bmatrix}
1 & 1 & |1 \\
2 & 3 & |1
\end{bmatrix}
\\

[\vec{v}_{2}]=? \\ 
\begin{bmatrix}
1 & 1 & |1 \\
2 & 3 & |-1
\end{bmatrix} \\
\begin{bmatrix}
1 & 1 & |1 & 1 \\
2 & 3 & |1 & -1
\end{bmatrix}\implies\begin{bmatrix}
1 & 0 & |2 & 4 \\
0 & 1 & |-1 & -3
\end{bmatrix} \\
P_{B\to C}=\begin{bmatrix}
2 & 4 \\
-1 & -3
\end{bmatrix} \\
\end{align}
$$
- ###### We just find each matrix and solve for the coordinates of the original ones
- #### The determinant of a change of basis matrix cannot be 0